examples/ghc/manual/Outputable.v
@@ -17,3 +17,30 @@ Class OutputableP (env : Type) (a : Type) := {}.
 Axiom SDoc : Type.
 
 Axiom braces : SDoc -> SDoc.
+Axiom colon : SDoc.
+Axiom NamePprCtx : Type.
+
+(* GHC 9.10: JoinPointHood moved from BasicTypes to a new GHC.Types.Basic *)
+Inductive JoinPointHood : Type :=
+  | NotJoinPoint : JoinPointHood
+  | JoinPoint : nat -> JoinPointHood.
+
+Require Import HsToCoq.Err.
+#[global] Instance Default__JoinPointHood : Default JoinPointHood :=
+  Build_Default _ NotJoinPoint.
+
+#[global] Definition isJoinPoint : JoinPointHood -> bool :=
+  fun jph => match jph with | JoinPoint _ => true | NotJoinPoint => false end.
+
+#[global] Instance Eq___JoinPointHood : Eq_ JoinPointHood :=
+  fun _ k => k (Eq___Dict_Build _
+    (fun x y => match x, y with
+    | NotJoinPoint, NotJoinPoint => true
+    | JoinPoint n, JoinPoint m => Nat.eqb n m
+    | _, _ => false
+    end)
+    (fun x y => match x, y with
+    | NotJoinPoint, NotJoinPoint => false
+    | JoinPoint n, JoinPoint m => negb (Nat.eqb n m)
+    | _, _ => true
+    end)).
