examples/ghc/lib/UnVarGraph.v
@@ -33,13 +33,13 @@ Inductive UnVarGraph : Type :=
 
 (* Midamble *)
 
-Instance Default_UnVarSet : HsToCoq.Err.Default UnVarSet :=
+#[global] Instance Default_UnVarSet : HsToCoq.Err.Default UnVarSet :=
   HsToCoq.Err.Build_Default _ (Mk_UnVarSet HsToCoq.Err.default).
-Instance Default_UnVarGraph : HsToCoq.Err.Default UnVarGraph :=
+#[global] Instance Default_UnVarGraph : HsToCoq.Err.Default UnVarGraph :=
   HsToCoq.Err.Build_Default _ (CG HsToCoq.Err.default).
 
 
-Instance Unpeel_UnVarSet : HsToCoq.Unpeel.Unpeel UnVarSet Data.IntSet.Internal.IntSet :=
+#[global] Instance Unpeel_UnVarSet : HsToCoq.Unpeel.Unpeel UnVarSet Data.IntSet.Internal.IntSet :=
   HsToCoq.Unpeel.Build_Unpeel _ _ (fun x => match x with | Mk_UnVarSet y => y end) Mk_UnVarSet.
 
 (* Converted value declarations: *)
