examples/ghc/lib/RepType.v
@@ -2,3 +2,5 @@
 Require AxiomatizedTypes.
 
 Axiom isZeroBitTy : AxiomatizedTypes.Type_ -> bool.
+Axiom PrimRep : Type.
+Axiom typePrimRep : AxiomatizedTypes.Type_ -> list PrimRep.
