examples/ghc/manual/GHC/Types/Cpr.v
@@ -6,4 +6,8 @@ Axiom topCprSig : CprSig.
 
 Axiom prependArgsCprSig : nat -> CprSig -> CprSig.
 
+Axiom CprType : Type.
+Axiom botCpr : CprType.
+Axiom mkCprSig : nat -> CprType -> CprSig.
+
 #[global] Instance Default__CprSig : HsToCoq.Err.Default CprSig. Admitted.
